Expand opon invariants

solutions/invariants.v
@@ -1,6 +1,12 @@
 From iris.base_logic.lib Require Export invariants.
 From iris.heap_lang Require Import lang proofmode notation.
 
+(*
+  Let's make a simple multi-threaded program. We can use `Fork e` to
+  create a new thread to run `e`. As such the following program will
+  race to either update `l` or read `l`. Meaning the resulting value
+  could be either 0 or 1.
+*)
 Definition prog : expr :=
   let: "l" := ref #0 in
   Fork ("l" <- #1);;
@@ -9,7 +15,42 @@ Definition prog : expr :=
 Section proofs.
 Context `{!heapGS Σ}.
 
+Lemma wp_prog : {{{ True }}} prog {{{ v, RET v; ⌜v = #0⌝ ∨ ⌜v = #1⌝ }}}.
+Proof.
+  iIntros "%Φ _ HΦ".
+  rewrite /prog.
+  wp_alloc l as "Hl".
+  wp_pures.
+  (*
+    Fork does not have its own tactic. Instead we use its
+    specification. This specification forces us to split our resources
+    between the threads.
+  *)
+  wp_apply (wp_fork with "[Hl]").
+  (*
+    As such we have to pick a thread to own `l`. But as both threads
+    need to access `l`, we are stuck.
+  *)
+Abort.
+
+(*
+  To get around this, we will use invariants. Invariants are written
+  `inv N P` where N is a namespace (Think of it as the name of the
+  invariant), and `P` is the proposition we want to make invariant.
+  As the name suggests, invariants are propositions that will remain
+  true forever. This allows them to be persistent no matter what P is.
+  
+  As stated, invariant need a namespace. This allows invariants to be
+  used together as long as they are in different namespaces.
+*)
 Let N := nroot .@ "stuff".
+
+(*
+  In this case we want the invariant to incapsulate ownership of `l`
+  as well as its posible values.
+*)
+Definition prog_inv (l : loc) : iProp Σ :=
+  ∃ v, l ↦ v ∗ (⌜v = #0⌝ ∨ ⌜v = #1⌝).
 
 Lemma wp_prog : {{{ True }}} prog {{{ v, RET v; ⌜v = #0⌝ ∨ ⌜v = #1⌝ }}}.
 Proof.
@@ -17,15 +58,35 @@ Proof.
   rewrite /prog.
   wp_alloc l as "Hl".
   wp_pures.
-  iMod (inv_alloc N _ (∃ v, l ↦ v ∗ (⌜v = #0⌝ ∨ ⌜v = #1⌝)) with "[Hl]") as "#I".
+  (*
+    To create an invariant we use the lemma
+    `inv_alloc : ▷P -∗ |={E}=> inv N P`.
+    In order to deal with the udpdate modality, we will use the iMod
+    tactic rather than iPoseProof or iDestruct.
+  *)
+  iMod (inv_alloc N _ (prog_inv l) with "[Hl]") as "#I".
   {
     iNext.
     iExists #0.
     iFrame.
     by iLeft.
   }
+  (*
+    As the invariant is persistent, we can now share it between the
+    threads.
+  *)
   wp_apply wp_fork.
-  - iInv "I" as "(%v & Hl & _)".
+  - (*
+      We can use the `iInv` to access the resources in the invariant.
+    *)
+    iInv "I" as "(%v & Hl & _)".
+    (*
+      Opening invariants have certain restrictions. It is only
+      posible to open invariants over an atomic step, and after this
+      step, we must reestablish the invariant.
+      Further more, the `@ ⊤ \ ↑N`, signifies that the `N` namespace
+      has been opened. As such we wont be able to open it twice at the same step.
+    *)
     wp_store.
     iSplitL; last done.
     iIntros "!> !>".
@@ -40,6 +101,92 @@ Proof.
     + iExists v.
       by iFrame.
     + by iApply "HΦ".
+Qed.
+
+End proofs.
+
+(*
+  Let's look at another program. This program will create a thread to
+  increment a counter. While the main thread will read the counter at
+  some point. As such, this program should produce some none negative
+  number. However, we will only prove that it returns a number.
+*)
+Definition prog2 : expr :=
+  let: "l" := ref #0 in
+  Fork ((
+    rec: "go" <> :=
+      "l" <- !"l" + #1;;
+      "go" #()
+  ) #());;
+  !"l".
+
+Section proofs.
+Context `{!heapGS Σ}.
+Let N := nroot .@ "other stuff".
+
+(*
+  Our invariant wil simply be that the location points to an integer.
+*)
+Definition prog2_inv (l : loc) : iProp Σ :=
+  ∃ i : Z, l ↦ #i.
+
+Lemma prog2_spec : {{{ True }}} prog2 {{{ (i : Z), RET #i; True }}}.
+Proof.
+  iIntros "%Φ _ HΦ".
+  rewrite /prog2.
+  wp_alloc l as "Hl".
+  wp_pures.
+  (*
+    Like before, we allocate the invariant.
+  *)
+  iMod (inv_alloc N _ (prog2_inv l) with "[Hl]") as "#I".
+  { iNext. by iExists 0. }
+  wp_apply wp_fork.
+  - wp_pure.
+    (* We use löb induction to accent the recursive calls *)
+    iLöb as "IH".
+    wp_pures.
+    (* If we now try to open the invariant: *)
+    iInv "I" as "[%i Hl]".
+    (*
+      We run into something different to earlier. This new subgoal
+      `Atomic` is a typeclass, stating that the program should only
+      consist of a single atomic operation. In this case the typeclass
+      search fails, because the program infact consists of two
+      operations. So it is not atomic.
+    *)
+    Undo.
+    (*
+      To get around this, we will use wp_bind to split the program
+      into atomic parts.
+      Notice that the %E is necesary to use the notation.
+    *)
+    wp_bind (! _)%E.
+    iInv "I" as "[%i Hl]".
+    wp_load.
+    iModIntro.
+    iSplitL "Hl".
+    { by iExists i. }
+    wp_pures.
+    (*
+      As we know need access to `l` again, we have to do the same
+      trick again.
+    *)
+    wp_bind (_ <- _)%E.
+    iInv "I" as "[%j Hl]".
+    wp_store.
+    iModIntro.
+    iSplitL "Hl".
+    { by iExists (i + 1)%Z. }
+    do 2 wp_pure.
+    done.
+  - wp_pures.
+    iInv "I" as "[%i Hl]".
+    wp_load.
+    iModIntro.
+    iSplitL "Hl".
+    { by iExists i. }
+    by iApply "HΦ".
 Qed.
 
 End proofs.
